Impl/CommitterCommitImpl.i.dfy
@@ -1,0 +1,139 @@
+include "CommitterImpl.i.dfy"
+include "CommitterCommitModel.i.dfy"
+
+module CommitterCommitImpl {
+  import opened NativeTypes
+  import opened Options
+
+  import opened DiskLayout
+  import JC = JournalCache
+  import opened Journal
+  import opened JournalBytes
+  import SectorType
+  import MutableMapModel
+
+  import opened CommitterImpl
+  import CommitterCommitModel
+
+  // TODO we could have these do the modification in-place instead.
+
+  method SyncReqs2to1(m: MutableMap.ResizingHashMap<JC.SyncReqStatus>)
+  returns (m' : MutableMap.ResizingHashMap<JC.SyncReqStatus>)
+  requires m.Inv()
+  ensures fresh(m'.Repr)
+  ensures m'.Inv()
+  ensures m'.I() == CommitterCommitModel.SyncReqs2to1(m.I())
+  {
+    CommitterCommitModel.reveal_SyncReqs2to1();
+    var it := m.IterStart();
+    var m0 := new MutableMap.ResizingHashMap(128);
+    while !it.next.Done?
+    invariant m.Inv()
+    invariant fresh(m0.Repr)
+    invariant m0.Inv()
+    invariant MutableMapModel.WFIter(m.I(), it)
+    invariant m0.Inv()
+    invariant m0.I().contents.Keys == it.s
+    invariant CommitterCommitModel.SyncReqs2to1(m.I()) == CommitterCommitModel.SyncReqs2to1Iterate(m.I(), it, m0.I())
+
+    decreases it.decreaser
+    {
+      MutableMapModel.LemmaIterIndexLtCount(m.I(), it);
+      MutableMapModel.CountBound(m.I());
+      m0.Insert(it.next.key, (if it.next.value == JC.State2 then JC.State1 else it.next.value));
+      it := m.IterInc(it);
+    }
+    m' := m0;
+  }
+
+
+  method SyncReqs3to2(m: MutableMap.ResizingHashMap<JC.SyncReqStatus>)
+  returns (m' : MutableMap.ResizingHashMap<JC.SyncReqStatus>)
+  requires m.Inv()
+  ensures fresh(m'.Repr)
+  ensures m'.Inv()
+  ensures m'.I() == CommitterCommitModel.SyncReqs3to2(m.I())
+  {
+    CommitterCommitModel.reveal_SyncReqs3to2();
+    var it := m.IterStart();
+    var m0 := new MutableMap.ResizingHashMap(128);
+    while !it.next.Done?
+    invariant m.Inv()
+    invariant fresh(m0.Repr)
+    invariant m0.Inv()
+    invariant MutableMapModel.WFIter(m.I(), it)
+    invariant m0.Inv()
+    invariant m0.I().contents.Keys == it.s
+    invariant CommitterCommitModel.SyncReqs3to2(m.I()) == CommitterCommitModel.SyncReqs3to2Iterate(m.I(), it, m0.I())
+
+    decreases it.decreaser
+    {
+      MutableMapModel.LemmaIterIndexLtCount(m.I(), it);
+      MutableMapModel.CountBound(m.I());
+      m0.Insert(it.next.key, (if it.next.value == JC.State3 then JC.State2 else it.next.value));
+      it := m.IterInc(it);
+    }
+    m' := m0;
+  }
+
+  method WriteOutJournal(k: ImplConstants, cm: Committer, io: DiskIOHandler)
+  requires io.initialized()
+  requires cm.Inv()
+  requires JournalistModel.I(cm.I().journalist).inMemoryJournalFrozen != []
+        || JournalistModel.I(cm.I().journalist).inMemoryJournal != []
+  modifies cm.Repr
+  ensures forall o | o in cm.Repr :: o in old(cm.Repr) || fresh(o)
+  ensures cm.Inv()
+  ensures cm.I() == CommitterCommitModel.WriteOutJournal(
+      k, old(cm.I()), IIO(io))
+  /*{
+    var writtenJournalLen :=
+        JournalistModel.getWrittenJournalLen(cm.journalist);
+
+    var doingFrozen :=
+      JournalistModel.hasFrozenJournal(cm.journalist);
+
+    var (journalist', j) :=
+      if doingFrozen then
+        JournalistModel.packageFrozenJournal(cm.journalist)
+      else
+        JournalistModel.packageInMemoryJournal(cm.journalist);
+
+    var start := start_pos_add(
+        cm.superblock.journalStart,
+        writtenJournalLen);
+
+    var len := |j| as uint64 / 4096;
+
+    var contiguous := start + len <= NumJournalBlocks();
+
+    var io' := if contiguous then
+      IOReqWrite(io.id, D.ReqWrite(JournalPoint(start), j))
+    else (
+      var cut := (NumJournalBlocks() - start) * 4096;
+      IOReqWrite2(io.id, io.id2,
+          D.ReqWrite(JournalPoint(start), j[..cut]),
+          D.ReqWrite(JournalPoint(0), j[cut..]))
+    );
+
+    var outstandingJournalWrites' := if contiguous
+        then cm.outstandingJournalWrites + {io.id}
+        else cm.outstandingJournalWrites + {io.id, io.id2};
+
+    var frozenJournalPosition' := if doingFrozen
+      then JournalistModel.getWrittenJournalLen(journalist')
+      else cm.frozenJournalPosition;
+
+    var syncReqs' := if doingFrozen
+      then cm.syncReqs
+      else SyncReqs3to2(cm.syncReqs);
+
+    var cm' := cm
+      .(outstandingJournalWrites := outstandingJournalWrites')
+      .(journalist := journalist')
+      .(frozenJournalPosition := frozenJournalPosition')
+      .(syncReqs := syncReqs');
+
+    (cm', io')
+  }*/
+}
